<?xml version="1.0"?>
<rdf:RDF xmlns="http://example.org/chi2025#"
     xml:base="http://example.org/chi2025"
     xmlns:ns="http://www.w3.org/2006/vcard/ns#"
     xmlns:org="http://www.w3.org/ns/org#"
     xmlns:owl="http://www.w3.org/2002/07/owl#"
     xmlns:rdf="http://www.w3.org/1999/02/22-rdf-syntax-ns#"
     xmlns:xml="http://www.w3.org/XML/1998/namespace"
     xmlns:xsd="http://www.w3.org/2001/XMLSchema#"
     xmlns:bibo="http://purl.org/ontology/bibo/"
     xmlns:chi1="http://example.org/chi2025#"
     xmlns:foaf="http://xmlns.com/foaf/0.1/"
     xmlns:hcio="urn:absolute:dev.nemo.inf.ufes.br/hcion/HCIO.owl#"
     xmlns:rdfs="http://www.w3.org/2000/01/rdf-schema#"
     xmlns:skos="http://www.w3.org/2004/02/skos/core#"
     xmlns:terms="http://purl.org/dc/terms/"
     xmlns:schema="http://schema.org/">
    <owl:Ontology rdf:about="http://example.org/chi2025">
        <owl:versionIRI rdf:resource="http://example.org/chi2025/1.0"/>
        <owl:imports rdf:resource="http://example.org/chi/instances"/> 
        <owl:imports rdf:resource="urn:absolute:dev.nemo.inf.ufes.br/hcion/HCIO.owl#/1.0"/>
        <rdfs:label>CHI 2025 Ontology</rdfs:label>
    </owl:Ontology>
    


    <!-- 
    ///////////////////////////////////////////////////////////////////////////////////////
    //
    // Object Properties
    //
    ///////////////////////////////////////////////////////////////////////////////////////
     -->

    


    <!-- http://example.org/chi2025#aboutTopic -->

    <owl:ObjectProperty rdf:about="http://example.org/chi2025#aboutTopic">
        <owl:inverseOf rdf:resource="http://example.org/chi2025#isTopicOf"/>
        <rdfs:domain rdf:resource="http://example.org/chi2025#Paper"/>
        <rdfs:range rdf:resource="http://example.org/chi2025#TopicConcept"/>
    </owl:ObjectProperty>
    


    <!-- http://example.org/chi2025#addressesIntention -->

    <owl:ObjectProperty rdf:about="http://example.org/chi2025#addressesIntention">
        <owl:inverseOf rdf:resource="http://example.org/chi2025#isAddressedBy"/>
        <rdfs:domain>
            <owl:Class>
                <owl:unionOf rdf:parseType="Collection">
                    <rdf:Description rdf:about="http://example.org/chi2025#SoftwareArtifact"/>
                    <rdf:Description rdf:about="http://example.org/chi2025#Study"/>
                </owl:unionOf>
            </owl:Class>
        </rdfs:domain>
        <rdfs:range rdf:resource="http://example.org/chi2025#IntentionSpecification"/>
    </owl:ObjectProperty>
    


    <!-- http://example.org/chi2025#affiliatedWith -->

    <owl:ObjectProperty rdf:about="http://example.org/chi2025#affiliatedWith">
        <owl:inverseOf rdf:resource="http://example.org/chi2025#hasMember"/>
        <rdfs:domain rdf:resource="http://example.org/chi2025#Author"/>
        <rdfs:range rdf:resource="http://example.org/chi2025#Affiliation"/>
    </owl:ObjectProperty>
    


    <!-- http://example.org/chi2025#affiliation -->

    <owl:ObjectProperty rdf:about="http://example.org/chi2025#affiliation">
        <rdfs:domain rdf:resource="http://example.org/chi2025#Authorship"/>
        <rdfs:range rdf:resource="http://www.w3.org/ns/org#Organization"/>
        <rdfs:label>affiliation (organization @ time of paper)</rdfs:label>
    </owl:ObjectProperty>
    


    <!-- http://example.org/chi2025#aimsAtGoal -->

    <owl:ObjectProperty rdf:about="http://example.org/chi2025#aimsAtGoal">
        <owl:inverseOf rdf:resource="http://example.org/chi2025#isGoalOf"/>
        <rdfs:domain>
            <owl:Class>
                <owl:unionOf rdf:parseType="Collection">
                    <rdf:Description rdf:about="http://example.org/chi2025#SoftwareArtifact"/>
                    <rdf:Description rdf:about="http://example.org/chi2025#Study"/>
                </owl:unionOf>
            </owl:Class>
        </rdfs:domain>
        <rdfs:range rdf:resource="http://example.org/chi2025#GoalSpecification"/>
    </owl:ObjectProperty>
    


    <!-- http://example.org/chi2025#author -->

    <owl:ObjectProperty rdf:about="http://example.org/chi2025#author">
        <rdfs:domain rdf:resource="http://example.org/chi2025#Authorship"/>
        <rdfs:range rdf:resource="http://xmlns.com/foaf/0.1/Person"/>
        <rdfs:label>author (person)</rdfs:label>
    </owl:ObjectProperty>
    


    <!-- http://example.org/chi2025#hasAuthor -->

    <owl:ObjectProperty rdf:about="http://example.org/chi2025#hasAuthor">
        <rdfs:subPropertyOf rdf:resource="http://purl.org/dc/terms/creator"/>
        <rdfs:domain rdf:resource="http://example.org/chi2025#Paper"/>
        <rdfs:range rdf:resource="http://xmlns.com/foaf/0.1/Person"/>
        <owl:propertyChainAxiom rdf:parseType="Collection">
            <rdf:Description rdf:about="http://example.org/chi2025#hasAuthorship"/>
            <rdf:Description rdf:about="http://example.org/chi2025#author"/>
        </owl:propertyChainAxiom>
        <rdfs:label>has author (direct)</rdfs:label>
    </owl:ObjectProperty>
    


    <!-- http://example.org/chi2025#hasAuthorOrg -->

    <owl:ObjectProperty rdf:about="http://example.org/chi2025#hasAuthorOrg">
        <rdfs:domain rdf:resource="http://example.org/chi2025#Paper"/>
        <rdfs:range rdf:resource="http://www.w3.org/ns/org#Organization"/>
        <owl:propertyChainAxiom rdf:parseType="Collection">
            <rdf:Description rdf:about="http://example.org/chi2025#hasAuthorship"/>
            <rdf:Description rdf:about="http://example.org/chi2025#affiliation"/>
        </owl:propertyChainAxiom>
        <rdfs:label>has author organization (inferred)</rdfs:label>
    </owl:ObjectProperty>
    


    <!-- http://example.org/chi2025#hasAuthorship -->

    <owl:ObjectProperty rdf:about="http://example.org/chi2025#hasAuthorship">
        <owl:inverseOf rdf:resource="http://example.org/chi2025#ofPaper"/>
        <rdfs:domain rdf:resource="http://example.org/chi2025#Paper"/>
        <rdfs:range rdf:resource="http://example.org/chi2025#Authorship"/>
        <rdfs:label>has authorship node</rdfs:label>
    </owl:ObjectProperty>
    


    <!-- http://example.org/chi2025#hasDevice -->

    <owl:ObjectProperty rdf:about="http://example.org/chi2025#hasDevice">
        <owl:inverseOf rdf:resource="http://example.org/chi2025#isDeviceOf"/>
        <rdfs:domain rdf:resource="http://example.org/chi2025#SoftwareArtifact"/>
        <rdfs:range rdf:resource="http://example.org/chi2025#DeviceArtifact"/>
    </owl:ObjectProperty>
    


    <!-- http://example.org/chi2025#hasInputDevice -->

    <owl:ObjectProperty rdf:about="http://example.org/chi2025#hasInputDevice">
        <rdfs:subPropertyOf rdf:resource="http://example.org/chi2025#hasDevice"/>
        <owl:inverseOf rdf:resource="http://example.org/chi2025#isInputDeviceOf"/>
        <rdfs:domain rdf:resource="http://example.org/chi2025#SoftwareArtifact"/>
        <rdfs:range rdf:resource="http://example.org/chi2025#InputDeviceArtifact"/>
    </owl:ObjectProperty>
    


    <!-- http://example.org/chi2025#hasInterface -->

    <owl:ObjectProperty rdf:about="http://example.org/chi2025#hasInterface">
        <owl:inverseOf rdf:resource="http://example.org/chi2025#isInterfaceOf"/>
        <rdfs:domain rdf:resource="http://example.org/chi2025#SoftwareArtifact"/>
        <rdfs:range rdf:resource="http://example.org/chi2025#InterfaceArtifact"/>
    </owl:ObjectProperty>
    


    <!-- http://example.org/chi2025#hasMeasure -->

    <owl:ObjectProperty rdf:about="http://example.org/chi2025#hasMeasure">
        <owl:inverseOf rdf:resource="http://example.org/chi2025#isMeasureOf"/>
        <rdfs:domain rdf:resource="http://example.org/chi2025#Study"/>
        <rdfs:range rdf:resource="http://example.org/chi2025#Measure"/>
    </owl:ObjectProperty>
    


    <!-- http://example.org/chi2025#hasMember -->

    <owl:ObjectProperty rdf:about="http://example.org/chi2025#hasMember">
        <rdfs:domain rdf:resource="http://example.org/chi2025#Affiliation"/>
        <rdfs:range rdf:resource="http://example.org/chi2025#Author"/>
    </owl:ObjectProperty>
    


    <!-- http://example.org/chi2025#hasOutputDevice -->

    <owl:ObjectProperty rdf:about="http://example.org/chi2025#hasOutputDevice">
        <rdfs:subPropertyOf rdf:resource="http://example.org/chi2025#hasDevice"/>
        <owl:inverseOf rdf:resource="http://example.org/chi2025#isOutputDeviceOf"/>
        <rdfs:domain rdf:resource="http://example.org/chi2025#SoftwareArtifact"/>
        <rdfs:range rdf:resource="http://example.org/chi2025#OutputDeviceArtifact"/>
    </owl:ObjectProperty>
    


    <!-- http://example.org/chi2025#hasPaper -->

    <owl:ObjectProperty rdf:about="http://example.org/chi2025#hasPaper">
        <owl:inverseOf rdf:resource="http://example.org/chi2025#hasSession"/>
        <rdfs:domain rdf:resource="http://example.org/chi2025#Session"/>
        <rdfs:range rdf:resource="http://example.org/chi2025#Paper"/>
    </owl:ObjectProperty>
    


    <!-- http://example.org/chi2025#hasPaperInTrack -->

    <owl:ObjectProperty rdf:about="http://example.org/chi2025#hasPaperInTrack">
        <owl:inverseOf rdf:resource="http://example.org/chi2025#hasTrack"/>
        <rdfs:domain rdf:resource="http://example.org/chi2025#Track"/>
        <rdfs:range rdf:resource="http://example.org/chi2025#Paper"/>
    </owl:ObjectProperty>
    


    <!-- http://example.org/chi2025#hasPrimaryTopic -->

    <owl:ObjectProperty rdf:about="http://example.org/chi2025#hasPrimaryTopic">
        <rdfs:subPropertyOf rdf:resource="http://example.org/chi2025#aboutTopic"/>
        <owl:inverseOf rdf:resource="http://example.org/chi2025#isPrimaryTopicOf"/>
        <rdf:type rdf:resource="http://www.w3.org/2002/07/owl#FunctionalProperty"/>
        <rdfs:domain rdf:resource="http://example.org/chi2025#Paper"/>
        <rdfs:range rdf:resource="http://example.org/chi2025#TopicConcept"/>
    </owl:ObjectProperty>
    


    <!-- http://example.org/chi2025#hasSession -->

    <owl:ObjectProperty rdf:about="http://example.org/chi2025#hasSession">
        <rdfs:domain rdf:resource="http://example.org/chi2025#Paper"/>
        <rdfs:range rdf:resource="http://example.org/chi2025#Session"/>
    </owl:ObjectProperty>
    


    <!-- http://example.org/chi2025#hasTrack -->

    <owl:ObjectProperty rdf:about="http://example.org/chi2025#hasTrack">
        <rdfs:domain rdf:resource="http://example.org/chi2025#Paper"/>
        <rdfs:range rdf:resource="http://example.org/chi2025#Track"/>
    </owl:ObjectProperty>
    


    <!-- http://example.org/chi2025#involvesParticipationPattern -->

    <owl:ObjectProperty rdf:about="http://example.org/chi2025#involvesParticipationPattern">
        <owl:inverseOf rdf:resource="http://example.org/chi2025#isParticipationPatternIn"/>
        <rdfs:domain rdf:resource="http://example.org/chi2025#Study"/>
        <rdfs:range rdf:resource="http://example.org/chi2025#ParticipationPattern"/>
    </owl:ObjectProperty>
    


    <!-- http://example.org/chi2025#isAddressedBy -->

    <owl:ObjectProperty rdf:about="http://example.org/chi2025#isAddressedBy">
        <rdfs:domain rdf:resource="http://example.org/chi2025#IntentionSpecification"/>
        <rdfs:range>
            <owl:Class>
                <owl:unionOf rdf:parseType="Collection">
                    <rdf:Description rdf:about="http://example.org/chi2025#SoftwareArtifact"/>
                    <rdf:Description rdf:about="http://example.org/chi2025#Study"/>
                </owl:unionOf>
            </owl:Class>
        </rdfs:range>
    </owl:ObjectProperty>
    


    <!-- http://example.org/chi2025#isAuthorOf -->

    <owl:ObjectProperty rdf:about="http://example.org/chi2025#isAuthorOf">
        <rdfs:domain rdf:resource="http://example.org/chi2025#Author"/>
        <rdfs:range rdf:resource="http://example.org/chi2025#Paper"/>
    </owl:ObjectProperty>
    


    <!-- http://example.org/chi2025#isDeviceOf -->

    <owl:ObjectProperty rdf:about="http://example.org/chi2025#isDeviceOf">
        <rdfs:domain rdf:resource="http://example.org/chi2025#DeviceArtifact"/>
        <rdfs:range rdf:resource="http://example.org/chi2025#SoftwareArtifact"/>
    </owl:ObjectProperty>
    


    <!-- http://example.org/chi2025#isGoalOf -->

    <owl:ObjectProperty rdf:about="http://example.org/chi2025#isGoalOf">
        <rdfs:domain rdf:resource="http://example.org/chi2025#GoalSpecification"/>
        <rdfs:range>
            <owl:Class>
                <owl:unionOf rdf:parseType="Collection">
                    <rdf:Description rdf:about="http://example.org/chi2025#SoftwareArtifact"/>
                    <rdf:Description rdf:about="http://example.org/chi2025#Study"/>
                </owl:unionOf>
            </owl:Class>
        </rdfs:range>
    </owl:ObjectProperty>
    


    <!-- http://example.org/chi2025#isInputDeviceOf -->

    <owl:ObjectProperty rdf:about="http://example.org/chi2025#isInputDeviceOf">
        <rdfs:domain rdf:resource="http://example.org/chi2025#InputDeviceArtifact"/>
        <rdfs:range rdf:resource="http://example.org/chi2025#SoftwareArtifact"/>
    </owl:ObjectProperty>
    


    <!-- http://example.org/chi2025#isInstrumentOf -->

    <owl:ObjectProperty rdf:about="http://example.org/chi2025#isInstrumentOf">
        <owl:inverseOf rdf:resource="http://example.org/chi2025#usesInstrument"/>
        <rdfs:domain rdf:resource="http://example.org/chi2025#Instrument"/>
        <rdfs:range>
            <owl:Class>
                <owl:unionOf rdf:parseType="Collection">
                    <rdf:Description rdf:about="http://example.org/chi2025#Measure"/>
                    <rdf:Description rdf:about="http://example.org/chi2025#Study"/>
                </owl:unionOf>
            </owl:Class>
        </rdfs:range>
    </owl:ObjectProperty>
    


    <!-- http://example.org/chi2025#isInterfaceOf -->

    <owl:ObjectProperty rdf:about="http://example.org/chi2025#isInterfaceOf">
        <rdfs:domain rdf:resource="http://example.org/chi2025#InterfaceArtifact"/>
        <rdfs:range rdf:resource="http://example.org/chi2025#SoftwareArtifact"/>
    </owl:ObjectProperty>
    


    <!-- http://example.org/chi2025#isMeasureOf -->

    <owl:ObjectProperty rdf:about="http://example.org/chi2025#isMeasureOf">
        <rdfs:domain rdf:resource="http://example.org/chi2025#Measure"/>
        <rdfs:range rdf:resource="http://example.org/chi2025#Study"/>
    </owl:ObjectProperty>
    


    <!-- http://example.org/chi2025#isOutputDeviceOf -->

    <owl:ObjectProperty rdf:about="http://example.org/chi2025#isOutputDeviceOf">
        <rdfs:domain rdf:resource="http://example.org/chi2025#OutputDeviceArtifact"/>
        <rdfs:range rdf:resource="http://example.org/chi2025#SoftwareArtifact"/>
    </owl:ObjectProperty>
    


    <!-- http://example.org/chi2025#isParticipationPatternIn -->

    <owl:ObjectProperty rdf:about="http://example.org/chi2025#isParticipationPatternIn">
        <rdfs:domain rdf:resource="http://example.org/chi2025#ParticipationPattern"/>
        <rdfs:range rdf:resource="http://example.org/chi2025#Study"/>
    </owl:ObjectProperty>
    


    <!-- http://example.org/chi2025#isPrimaryTopicOf -->

    <owl:ObjectProperty rdf:about="http://example.org/chi2025#isPrimaryTopicOf">
        <rdfs:domain rdf:resource="http://example.org/chi2025#TopicConcept"/>
        <rdfs:range rdf:resource="http://example.org/chi2025#Paper"/>
    </owl:ObjectProperty>
    


    <!-- http://example.org/chi2025#isProposedIn -->

    <owl:ObjectProperty rdf:about="http://example.org/chi2025#isProposedIn">
        <owl:inverseOf rdf:resource="http://example.org/chi2025#proposesArtifact"/>
        <rdfs:domain rdf:resource="http://example.org/chi2025#SoftwareArtifact"/>
        <rdfs:range rdf:resource="http://example.org/chi2025#Paper"/>
    </owl:ObjectProperty>
    


    <!-- http://example.org/chi2025#isResultOf -->

    <owl:ObjectProperty rdf:about="http://example.org/chi2025#isResultOf">
        <owl:inverseOf rdf:resource="http://example.org/chi2025#reportsResult"/>
        <rdfs:domain rdf:resource="http://example.org/chi2025#Result"/>
        <rdfs:range rdf:resource="http://example.org/chi2025#Study"/>
    </owl:ObjectProperty>
    


    <!-- http://example.org/chi2025#isStudyReportedIn -->

    <owl:ObjectProperty rdf:about="http://example.org/chi2025#isStudyReportedIn">
        <owl:inverseOf rdf:resource="http://example.org/chi2025#paperIncludesStudy"/>
        <rdfs:domain rdf:resource="http://example.org/chi2025#Study"/>
        <rdfs:range rdf:resource="http://example.org/chi2025#Paper"/>
    </owl:ObjectProperty>
    


    <!-- http://example.org/chi2025#isTopicOf -->

    <owl:ObjectProperty rdf:about="http://example.org/chi2025#isTopicOf">
        <rdfs:domain rdf:resource="http://example.org/chi2025#TopicConcept"/>
        <rdfs:range rdf:resource="http://example.org/chi2025#Paper"/>
    </owl:ObjectProperty>
    


    <!-- http://example.org/chi2025#isTopicOfStudy -->

    <owl:ObjectProperty rdf:about="http://example.org/chi2025#isTopicOfStudy">
        <owl:inverseOf rdf:resource="http://example.org/chi2025#studyAboutTopic"/>
        <rdfs:domain rdf:resource="http://example.org/chi2025#TopicConcept"/>
        <rdfs:range rdf:resource="http://example.org/chi2025#Study"/>
    </owl:ObjectProperty>
    


    <!-- http://example.org/chi2025#ofPaper -->

    <owl:ObjectProperty rdf:about="http://example.org/chi2025#ofPaper">
        <rdfs:domain rdf:resource="http://example.org/chi2025#Authorship"/>
        <rdfs:range rdf:resource="http://example.org/chi2025#Paper"/>
        <rdfs:label>of paper</rdfs:label>
    </owl:ObjectProperty>
    


    <!-- http://example.org/chi2025#paperIncludesStudy -->

    <owl:ObjectProperty rdf:about="http://example.org/chi2025#paperIncludesStudy">
        <rdfs:domain rdf:resource="http://example.org/chi2025#Paper"/>
        <rdfs:range rdf:resource="http://example.org/chi2025#Study"/>
    </owl:ObjectProperty>
    


    <!-- http://example.org/chi2025#proposesArtifact -->

    <owl:ObjectProperty rdf:about="http://example.org/chi2025#proposesArtifact">
        <rdfs:domain rdf:resource="http://example.org/chi2025#Paper"/>
        <rdfs:range rdf:resource="http://example.org/chi2025#SoftwareArtifact"/>
    </owl:ObjectProperty>
    


    <!-- http://example.org/chi2025#relatedPaper -->

    <owl:ObjectProperty rdf:about="http://example.org/chi2025#relatedPaper">
        <rdf:type rdf:resource="http://www.w3.org/2002/07/owl#SymmetricProperty"/>
        <rdfs:domain rdf:resource="http://example.org/chi2025#Paper"/>
        <rdfs:range rdf:resource="http://example.org/chi2025#Paper"/>
    </owl:ObjectProperty>
    


    <!-- http://example.org/chi2025#reportsResult -->

    <owl:ObjectProperty rdf:about="http://example.org/chi2025#reportsResult">
        <rdfs:domain rdf:resource="http://example.org/chi2025#Study"/>
        <rdfs:range rdf:resource="http://example.org/chi2025#Result"/>
    </owl:ObjectProperty>
    


    <!-- http://example.org/chi2025#studyAboutTopic -->

    <owl:ObjectProperty rdf:about="http://example.org/chi2025#studyAboutTopic">
        <rdfs:subPropertyOf rdf:resource="http://example.org/chi2025#aboutTopic"/>
        <rdfs:domain rdf:resource="http://example.org/chi2025#Study"/>
        <rdfs:range rdf:resource="http://example.org/chi2025#TopicConcept"/>
    </owl:ObjectProperty>
    


    <!-- http://example.org/chi2025#usesInstrument -->

    <owl:ObjectProperty rdf:about="http://example.org/chi2025#usesInstrument">
        <rdfs:domain>
            <owl:Class>
                <owl:unionOf rdf:parseType="Collection">
                    <rdf:Description rdf:about="http://example.org/chi2025#Measure"/>
                    <rdf:Description rdf:about="http://example.org/chi2025#Study"/>
                </owl:unionOf>
            </owl:Class>
        </rdfs:domain>
        <rdfs:range rdf:resource="http://example.org/chi2025#Instrument"/>
    </owl:ObjectProperty>
    


    <!-- http://purl.org/dc/terms/creator -->

    <owl:ObjectProperty rdf:about="http://purl.org/dc/terms/creator"/>
    


    <!-- http://www.w3.org/2006/vcard/ns#hasAddress -->

    <owl:ObjectProperty rdf:about="http://www.w3.org/2006/vcard/ns#hasAddress">
        <rdfs:domain rdf:resource="http://www.w3.org/ns/org#Organization"/>
        <rdfs:range rdf:resource="http://www.w3.org/2006/vcard/ns#Address"/>
        <rdfs:label>has address</rdfs:label>
    </owl:ObjectProperty>
    


    <!-- http://www.w3.org/ns/org#memberOf -->

    <owl:ObjectProperty rdf:about="http://www.w3.org/ns/org#memberOf">
        <rdfs:domain rdf:resource="http://xmlns.com/foaf/0.1/Person"/>
        <rdfs:range rdf:resource="http://www.w3.org/ns/org#Organization"/>
        <rdfs:label>member of</rdfs:label>
    </owl:ObjectProperty>
    


    <!-- 
    ///////////////////////////////////////////////////////////////////////////////////////
    //
    // Data properties
    //
    ///////////////////////////////////////////////////////////////////////////////////////
     -->

    


    <!-- http://example.org/chi2025#orgType -->

    <owl:DatatypeProperty rdf:about="http://example.org/chi2025#orgType">
        <rdfs:domain rdf:resource="http://www.w3.org/ns/org#Organization"/>
        <rdfs:range rdf:resource="http://www.w3.org/2001/XMLSchema#string"/>
    </owl:DatatypeProperty>
    


    <!-- http://purl.org/dc/terms/abstract -->

    <owl:DatatypeProperty rdf:about="http://purl.org/dc/terms/abstract">
        <rdfs:domain rdf:resource="http://example.org/chi2025#Paper"/>
        <rdfs:range rdf:resource="http://www.w3.org/2001/XMLSchema#string"/>
    </owl:DatatypeProperty>
    


    <!-- http://purl.org/dc/terms/identifier -->

    <owl:DatatypeProperty rdf:about="http://purl.org/dc/terms/identifier">
        <rdfs:domain rdf:resource="http://example.org/chi2025#Paper"/>
        <rdfs:range rdf:resource="http://www.w3.org/2001/XMLSchema#string"/>
    </owl:DatatypeProperty>
    


    <!-- http://purl.org/dc/terms/title -->

    <owl:DatatypeProperty rdf:about="http://purl.org/dc/terms/title">
        <rdfs:domain rdf:resource="http://example.org/chi2025#Paper"/>
        <rdfs:range rdf:resource="http://www.w3.org/2001/XMLSchema#string"/>
    </owl:DatatypeProperty>
    


    <!-- http://www.w3.org/2006/vcard/ns#country-name -->

    <owl:DatatypeProperty rdf:about="http://www.w3.org/2006/vcard/ns#country-name">
        <rdfs:domain rdf:resource="http://www.w3.org/2006/vcard/ns#Address"/>
        <rdfs:range rdf:resource="http://www.w3.org/2001/XMLSchema#string"/>
    </owl:DatatypeProperty>
    


    <!-- http://www.w3.org/2006/vcard/ns#locality -->

    <owl:DatatypeProperty rdf:about="http://www.w3.org/2006/vcard/ns#locality">
        <rdfs:domain rdf:resource="http://www.w3.org/2006/vcard/ns#Address"/>
        <rdfs:range rdf:resource="http://www.w3.org/2001/XMLSchema#string"/>
    </owl:DatatypeProperty>
    


    <!-- http://www.w3.org/2006/vcard/ns#organization-name -->

    <owl:DatatypeProperty rdf:about="http://www.w3.org/2006/vcard/ns#organization-name">
        <rdfs:domain rdf:resource="http://www.w3.org/ns/org#Organization"/>
        <rdfs:range rdf:resource="http://www.w3.org/2001/XMLSchema#string"/>
    </owl:DatatypeProperty>
    


    <!-- http://www.w3.org/2006/vcard/ns#region -->

    <owl:DatatypeProperty rdf:about="http://www.w3.org/2006/vcard/ns#region">
        <rdfs:domain rdf:resource="http://www.w3.org/2006/vcard/ns#Address"/>
        <rdfs:range rdf:resource="http://www.w3.org/2001/XMLSchema#string"/>
    </owl:DatatypeProperty>
    


    <!-- 
    ///////////////////////////////////////////////////////////////////////////////////////
    //
    // Classes
    //
    ///////////////////////////////////////////////////////////////////////////////////////
     -->

    


    <!-- http://example.org/chi2025#Affiliation -->

    <owl:Class rdf:about="http://example.org/chi2025#Affiliation">
        <rdfs:comment xml:lang="en">An affiliation associated with an authorship, typically representing the organization with which an author is linked at the time of a CHI paper.</rdfs:comment>
    </owl:Class>
    


    <!-- http://example.org/chi2025#Author -->

    <owl:Class rdf:about="http://example.org/chi2025#Author">
        <rdfs:comment xml:lang="en">An author who contributes to a CHI paper and is represented through one or more authorship relations to that paper.</rdfs:comment>
    </owl:Class>
    


    <!-- http://example.org/chi2025#Authorship -->

    <owl:Class rdf:about="http://example.org/chi2025#Authorship">
        <rdfs:subClassOf>
            <owl:Restriction>
                <owl:onProperty rdf:resource="http://example.org/chi2025#affiliation"/>
                <owl:someValuesFrom rdf:resource="http://www.w3.org/ns/org#Organization"/>
            </owl:Restriction>
        </rdfs:subClassOf>
        <rdfs:subClassOf>
            <owl:Restriction>
                <owl:onProperty rdf:resource="http://example.org/chi2025#author"/>
                <owl:qualifiedCardinality rdf:datatype="http://www.w3.org/2001/XMLSchema#nonNegativeInteger">1</owl:qualifiedCardinality>
                <owl:onClass rdf:resource="http://xmlns.com/foaf/0.1/Person"/>
            </owl:Restriction>
        </rdfs:subClassOf>
        <rdfs:subClassOf>
            <owl:Restriction>
                <owl:onProperty rdf:resource="http://example.org/chi2025#ofPaper"/>
                <owl:qualifiedCardinality rdf:datatype="http://www.w3.org/2001/XMLSchema#nonNegativeInteger">1</owl:qualifiedCardinality>
                <owl:onClass rdf:resource="http://example.org/chi2025#Paper"/>
            </owl:Restriction>
        </rdfs:subClassOf>
        <rdfs:comment xml:lang="en">A reified authorship relation that links exactly one person, one paper, and at least one organization affiliation for that author.</rdfs:comment>
    </owl:Class>
    


    <!-- http://example.org/chi2025#BaselineComparisonStudy -->

    <owl:Class rdf:about="http://example.org/chi2025#BaselineComparisonStudy">
        <rdfs:subClassOf rdf:resource="http://example.org/chi2025#Study"/>
        <rdfs:comment xml:lang="en">A study that compares a proposed system or condition against one or more baseline conditions to assess relative performance or effects.</rdfs:comment>
    </owl:Class>
    


    <!-- http://example.org/chi2025#DeviceArtifact -->

    <owl:Class rdf:about="http://example.org/chi2025#DeviceArtifact">
        <rdfs:subClassOf rdf:resource="urn:absolute:dev.nemo.inf.ufes.br/hcion/HCIO.owl#Hardware_Equipment"/>
        <rdfs:comment xml:lang="en">A hardware device used in an interactive system or study, such as an input or output device associated with a software artifact.</rdfs:comment>
    </owl:Class>
    


    <!-- http://example.org/chi2025#DiaryStudy -->

    <owl:Class rdf:about="http://example.org/chi2025#DiaryStudy">
        <rdfs:subClassOf rdf:resource="http://example.org/chi2025#QualitativeStudy"/>
        <rdfs:comment xml:lang="en">A qualitative study in which participants keep diaries or logs of their experiences or behaviors over time.</rdfs:comment>
    </owl:Class>
    


    <!-- http://example.org/chi2025#FieldStudy -->

    <owl:Class rdf:about="http://example.org/chi2025#FieldStudy">
        <rdfs:subClassOf rdf:resource="http://example.org/chi2025#Study"/>
        <rdfs:comment xml:lang="en">A study conducted in real-world settings, observing participants using systems or interventions in their natural context.</rdfs:comment>
    </owl:Class>
    


    <!-- http://example.org/chi2025#FocusGroupDiscussion -->

    <owl:Class rdf:about="http://example.org/chi2025#FocusGroupDiscussion">
        <rdfs:subClassOf rdf:resource="http://example.org/chi2025#QualitativeStudy"/>
        <rdfs:comment xml:lang="en">A qualitative study method in which a group of participants discuss topics or designs together under facilitation.</rdfs:comment>
    </owl:Class>
    


    <!-- http://example.org/chi2025#FormativeInterview -->

    <owl:Class rdf:about="http://example.org/chi2025#FormativeInterview">
        <rdfs:subClassOf rdf:resource="http://example.org/chi2025#InterviewStudy"/>
        <rdfs:comment xml:lang="en">An interview-based study conducted primarily to inform or shape the design, requirements, or research questions of subsequent work.</rdfs:comment>
    </owl:Class>
    


    <!-- http://example.org/chi2025#GoalSpecification -->

    <owl:Class rdf:about="http://example.org/chi2025#GoalSpecification">
        <rdfs:subClassOf rdf:resource="urn:absolute:dev.nemo.inf.ufes.br/hcion/HCIO.owl#User_Goal"/>
        <rdfs:comment xml:lang="en">A specification of a user goal that an interactive system or study aims to satisfy or support.</rdfs:comment>
    </owl:Class>
    


    <!-- http://example.org/chi2025#InputDeviceArtifact -->

    <owl:Class rdf:about="http://example.org/chi2025#InputDeviceArtifact">
        <rdfs:subClassOf rdf:resource="urn:absolute:dev.nemo.inf.ufes.br/hcion/HCIO.owl#Input_Equipment"/>
        <rdfs:comment xml:lang="en">A hardware device used primarily for user input in an interactive system, such as keyboard, touch, or sensors.</rdfs:comment>
    </owl:Class>
    


    <!-- http://example.org/chi2025#Instrument -->

    <owl:Class rdf:about="http://example.org/chi2025#Instrument">
        <rdfs:comment xml:lang="en">A data collection instrument used in a study, such as a logging setup, questionnaire, or sensor-based apparatus.</rdfs:comment>
    </owl:Class>
    
    <!-- ============================
        Instrument Subclasses
    =============================== -->

    <!-- Sensor Instruments -->

    <owl:Class rdf:about="http://example.org/chi2025#EyeTracker">
        <rdfs:subClassOf rdf:resource="http://example.org/chi2025#SensorInstrument"/>
        <rdfs:label>Eye Tracker</rdfs:label>
        <rdfs:comment xml:lang="en">A sensor-based instrument that measures users&apos; gaze or eye movements during interaction or experimental tasks.</rdfs:comment>
    </owl:Class>

    <owl:Class rdf:about="http://example.org/chi2025#WearableSensor">
        <rdfs:subClassOf rdf:resource="http://example.org/chi2025#SensorInstrument"/>
        <rdfs:label>Wearable Sensor</rdfs:label>
        <rdfs:comment xml:lang="en">A sensor instrument worn on the body to capture physiological or behavioral signals relevant to a study.</rdfs:comment>
    </owl:Class>

    <owl:Class rdf:about="http://example.org/chi2025#SmartwatchSensor">
        <rdfs:subClassOf rdf:resource="http://example.org/chi2025#SensorInstrument"/>
        <rdfs:label>Smartwatch Sensor</rdfs:label>
        <rdfs:comment xml:lang="en">A wearable sensor embedded in a smartwatch that collects usage, activity, or physiological data in a study.</rdfs:comment>
    </owl:Class>


    <!-- http://example.org/chi2025#IntentionSpecification -->

    <owl:Class rdf:about="http://example.org/chi2025#IntentionSpecification">
        <rdfs:subClassOf rdf:resource="urn:absolute:dev.nemo.inf.ufes.br/hcion/HCIO.owl#User_Intention"/>
        <rdfs:comment xml:lang="en">A specification of a user intention or desired behavior that an interactive system or intervention is designed to address.</rdfs:comment>
    </owl:Class>
    


    <!-- http://example.org/chi2025#InterfaceArtifact -->

    <owl:Class rdf:about="http://example.org/chi2025#InterfaceArtifact">
        <rdfs:subClassOf rdf:resource="urn:absolute:dev.nemo.inf.ufes.br/hcion/HCIO.owl#User_Interface"/>
        <rdfs:comment xml:lang="en">A user interface component or configuration that mediates interaction between a user and a software artifact.</rdfs:comment>
    </owl:Class>
    


    <!-- http://example.org/chi2025#InterviewStudy -->

    <owl:Class rdf:about="http://example.org/chi2025#InterviewStudy">
        <rdfs:subClassOf rdf:resource="http://example.org/chi2025#QualitativeStudy"/>
        <rdfs:comment xml:lang="en">A qualitative study that collects data primarily through structured, semi-structured, or unstructured interviews with participants.</rdfs:comment>
    </owl:Class>
    


    <!-- http://example.org/chi2025#LoggingInstrumentation -->

    <owl:Class rdf:about="http://example.org/chi2025#LoggingInstrumentation">
        <rdfs:subClassOf rdf:resource="http://example.org/chi2025#Instrument"/>
        <rdfs:comment xml:lang="en">An instrument that records interaction traces or usage logs of a system, typically in the background.</rdfs:comment>
    </owl:Class>
    


    <!-- http://example.org/chi2025#Measure -->

    <owl:Class rdf:about="http://example.org/chi2025#Measure">
        <rdfs:comment xml:lang="en">A variable or quantity assessed in a study to capture outcomes, behaviors, or experiences of interest.</rdfs:comment>
    </owl:Class>
    

    <!-- ============================
        Measure Subclasses
    =============================== -->

    <owl:Class rdf:about="http://example.org/chi2025#ReactionTimeMeasure">
        <rdfs:subClassOf rdf:resource="http://example.org/chi2025#PerformanceMeasure"/>
        <rdfs:label>Reaction Time Measure</rdfs:label>
        <rdfs:comment xml:lang="en">A performance measure that captures the time users take to respond to stimuli or complete specific actions.</rdfs:comment>
    </owl:Class>

    <owl:Class rdf:about="http://example.org/chi2025#CompletionTimeMeasure">
        <rdfs:subClassOf rdf:resource="http://example.org/chi2025#PerformanceMeasure"/>
        <rdfs:label>Completion Time Measure</rdfs:label>
        <rdfs:comment xml:lang="en">A performance measure that records how long it takes users to complete tasks or workflows.</rdfs:comment>
    </owl:Class>

    <owl:Class rdf:about="http://example.org/chi2025#ErrorRateMeasure">
        <rdfs:subClassOf rdf:resource="http://example.org/chi2025#PerformanceMeasure"/>
        <rdfs:label>Error Rate Measure</rdfs:label>
        <rdfs:comment xml:lang="en">A performance measure that quantifies how frequently users make errors while performing tasks.</rdfs:comment>
    </owl:Class>

    <owl:Class rdf:about="http://example.org/chi2025#AccuracyMeasure">
        <rdfs:subClassOf rdf:resource="http://example.org/chi2025#PerformanceMeasure"/>
        <rdfs:label>Accuracy Measure</rdfs:label>
        <rdfs:comment xml:lang="en">A performance measure that assesses how correct or precise users&apos; responses or task outcomes are.</rdfs:comment>
    </owl:Class>


    <!-- Subjective -->

    <owl:Class rdf:about="http://example.org/chi2025#LikertScaleMeasure">
        <rdfs:subClassOf rdf:resource="http://example.org/chi2025#SubjectiveMeasure"/>
        <rdfs:label>Likert Scale Measure</rdfs:label>
        <rdfs:comment xml:lang="en">A subjective measure based on Likert-scale responses, typically capturing attitudes, agreement, or perceived experience.</rdfs:comment>
    </owl:Class>

    <owl:Class rdf:about="http://example.org/chi2025#UsabilityRatingMeasure">
        <rdfs:subClassOf rdf:resource="http://example.org/chi2025#SubjectiveMeasure"/>
        <rdfs:label>Usability Rating Measure</rdfs:label>
        <rdfs:comment xml:lang="en">A subjective measure that captures users&apos; ratings of a system&apos;s usability or user experience quality.</rdfs:comment>
    </owl:Class>


    <!-- Physiological -->

    <owl:Class rdf:about="http://example.org/chi2025#HeartRateMeasure">
        <rdfs:subClassOf rdf:resource="http://example.org/chi2025#PhysiologicalMeasure"/>
        <rdfs:label>Heart Rate Measure</rdfs:label>
        <rdfs:comment xml:lang="en">A physiological measure that records heart rate or related cardiac signals as part of a study.</rdfs:comment>
    </owl:Class>


    <!-- http://example.org/chi2025#OutputDeviceArtifact -->

    <owl:Class rdf:about="http://example.org/chi2025#OutputDeviceArtifact">
        <rdfs:subClassOf rdf:resource="urn:absolute:dev.nemo.inf.ufes.br/hcion/HCIO.owl#Output_Equipment"/>
        <rdfs:comment xml:lang="en">A hardware device used primarily for presenting output from an interactive system, such as screens or speakers.</rdfs:comment>
    </owl:Class>
    


    <!-- http://example.org/chi2025#Paper -->

    <owl:Class rdf:about="http://example.org/chi2025#Paper">
        <rdfs:subClassOf rdf:resource="http://purl.org/ontology/bibo/Article"/>
        <rdfs:subClassOf>
            <owl:Restriction>
                <owl:onProperty rdf:resource="http://example.org/chi2025#hasAuthor"/>
                <owl:someValuesFrom rdf:resource="http://xmlns.com/foaf/0.1/Person"/>
            </owl:Restriction>
        </rdfs:subClassOf>
        <rdfs:label>CHI Paper</rdfs:label>
        <rdfs:comment xml:lang="en">A CHI research paper modeled as a bibliographic article that has one or more human authors and may report studies, measures, and results.</rdfs:comment>
    </owl:Class>
    


    <!-- http://example.org/chi2025#ParticipationPattern -->

    <owl:Class rdf:about="http://example.org/chi2025#ParticipationPattern">
        <rdfs:subClassOf rdf:resource="urn:absolute:dev.nemo.inf.ufes.br/hcion/HCIO.owl#User_Participation"/>
        <rdfs:comment xml:lang="en">A pattern describing how users participate in a system or study, such as in-the-wild usage or lab sessions.</rdfs:comment>
    </owl:Class>
    


    <!-- http://example.org/chi2025#PerformanceMeasure -->

    <owl:Class rdf:about="http://example.org/chi2025#PerformanceMeasure">
        <rdfs:subClassOf rdf:resource="http://example.org/chi2025#Measure"/>
        <rdfs:comment xml:lang="en">A measure that captures how well users perform tasks, often in terms of speed, accuracy, or efficiency.</rdfs:comment>
    </owl:Class>
    


    <!-- http://example.org/chi2025#PhysiologicalMeasure -->

    <owl:Class rdf:about="http://example.org/chi2025#PhysiologicalMeasure">
        <rdfs:subClassOf rdf:resource="http://example.org/chi2025#Measure"/>
        <rdfs:comment xml:lang="en">A measure based on physiological signals such as heart rate, skin conductance, or other bodily responses.</rdfs:comment>
    </owl:Class>
    


    <!-- http://example.org/chi2025#QualitativeResult -->

    <owl:Class rdf:about="http://example.org/chi2025#QualitativeResult">
        <rdfs:subClassOf rdf:resource="http://example.org/chi2025#Result"/>
        <rdfs:comment xml:lang="en">A result derived from qualitative analysis, such as themes, categories, or narratives about user experiences.</rdfs:comment>
    </owl:Class>
    


    <!-- http://example.org/chi2025#QualitativeStudy -->

    <owl:Class rdf:about="http://example.org/chi2025#QualitativeStudy">
        <rdfs:subClassOf rdf:resource="http://example.org/chi2025#Study"/>
        <owl:disjointWith rdf:resource="http://example.org/chi2025#QuantitativeStudy"/>
        <rdfs:comment xml:lang="en">A study that primarily uses qualitative methods, such as interviews, observations, or diary entries, to understand user experiences.</rdfs:comment>
    </owl:Class>
    


    <!-- http://example.org/chi2025#QuantitativeStudy -->

    <owl:Class rdf:about="http://example.org/chi2025#QuantitativeStudy">
        <rdfs:subClassOf rdf:resource="http://example.org/chi2025#Study"/>
        <rdfs:comment xml:lang="en">A study that primarily uses quantitative methods, such as experiments or surveys, and statistical analysis of numerical data.</rdfs:comment>
    </owl:Class>
    


    <!-- http://example.org/chi2025#Questionnaire -->

    <owl:Class rdf:about="http://example.org/chi2025#Questionnaire">
        <rdfs:subClassOf rdf:resource="http://example.org/chi2025#Instrument"/>
        <rdfs:comment xml:lang="en">An instrument that collects structured responses from participants through questions, often using scales or multiple-choice items.</rdfs:comment>
    </owl:Class>
    


    <!-- http://example.org/chi2025#Result -->

    <owl:Class rdf:about="http://example.org/chi2025#Result">
        <rdfs:comment xml:lang="en">An outcome produced by a study, such as findings, effect estimates, or qualitative insights.</rdfs:comment>
    </owl:Class>
    


    <!-- http://example.org/chi2025#SensorInstrument -->

    <owl:Class rdf:about="http://example.org/chi2025#SensorInstrument">
        <rdfs:subClassOf rdf:resource="http://example.org/chi2025#Instrument"/>
        <rdfs:comment xml:lang="en">An instrument that relies on sensors to capture signals or data from users or the environment.</rdfs:comment>
    </owl:Class>
    


    <!-- http://example.org/chi2025#Session -->

    <owl:Class rdf:about="http://example.org/chi2025#Session">
        <rdfs:comment xml:lang="en">A unit of time-bounded participation in a study or interaction with a system, often associated with specific tasks or conditions.</rdfs:comment>
    </owl:Class>
    


    <!-- http://example.org/chi2025#SoftwareArtifact -->

    <owl:Class rdf:about="http://example.org/chi2025#SoftwareArtifact">
        <rdfs:subClassOf rdf:resource="urn:absolute:dev.nemo.inf.ufes.br/hcion/HCIO.owl#Interactive_Computer_System"/>
        <rdfs:comment xml:lang="en">An interactive software system or prototype that users interact with and that may be evaluated in CHI studies.</rdfs:comment>
    </owl:Class>
    


    <!-- http://example.org/chi2025#StatisticalResult -->

    <owl:Class rdf:about="http://example.org/chi2025#StatisticalResult">
        <rdfs:subClassOf rdf:resource="http://example.org/chi2025#Result"/>
        <rdfs:comment xml:lang="en">A result expressed through statistical analysis, such as effect sizes, significance tests, or model estimates.</rdfs:comment>
    </owl:Class>
    


    <!-- http://example.org/chi2025#Study -->

    <owl:Class rdf:about="http://example.org/chi2025#Study">
        <rdfs:comment xml:lang="en">A research study reported in a CHI paper, which may involve users, interventions, measures, and results.</rdfs:comment>
    </owl:Class>
    


    <!-- http://example.org/chi2025#SubjectiveMeasure -->

    <owl:Class rdf:about="http://example.org/chi2025#SubjectiveMeasure">
        <rdfs:subClassOf rdf:resource="http://example.org/chi2025#Measure"/>
        <rdfs:comment xml:lang="en">A measure based on participants&apos; self-reported perceptions, feelings, or judgments rather than purely objective performance or signals.</rdfs:comment>
    </owl:Class>
    


    <!-- http://example.org/chi2025#SystemUsageInterview -->

    <owl:Class rdf:about="http://example.org/chi2025#SystemUsageInterview">
        <rdfs:subClassOf rdf:resource="http://example.org/chi2025#InterviewStudy"/>
        <rdfs:comment xml:lang="en">An interview-based study that focuses on how people use a particular system in their real or intended contexts.</rdfs:comment>
    </owl:Class>
    


    <!-- http://example.org/chi2025#ThinkAloudStudy -->

    <owl:Class rdf:about="http://example.org/chi2025#ThinkAloudStudy">
        <rdfs:subClassOf rdf:resource="http://example.org/chi2025#QualitativeStudy"/>
        <rdfs:comment xml:lang="en">A qualitative study in which participants verbalize their thoughts while interacting with a system or performing tasks.</rdfs:comment>
    </owl:Class>
    


    <!-- http://example.org/chi2025#TopicConcept -->

    <owl:Class rdf:about="http://example.org/chi2025#TopicConcept">
        <rdfs:subClassOf rdf:resource="http://www.w3.org/2004/02/skos/core#Concept"/>
        <rdfs:comment xml:lang="en">A topical concept that represents a CHI research theme or topic used to annotate papers and studies.</rdfs:comment>
    </owl:Class>
    


    <!-- http://example.org/chi2025#Track -->

    <owl:Class rdf:about="http://example.org/chi2025#Track">
        <rdfs:comment xml:lang="en">A track or category within the CHI conference to which papers can be assigned.</rdfs:comment>
    </owl:Class>
    


    <!-- http://example.org/chi2025#UsageScenarioInterview -->

    <owl:Class rdf:about="http://example.org/chi2025#UsageScenarioInterview">
        <rdfs:subClassOf rdf:resource="http://example.org/chi2025#InterviewStudy"/>
        <rdfs:comment xml:lang="en">An interview study that explores possible or actual scenarios of using a system, focusing on context and activities.</rdfs:comment>
    </owl:Class>
    


    <!-- http://example.org/chi2025#UserStudy -->

    <owl:Class rdf:about="http://example.org/chi2025#UserStudy">
        <rdfs:subClassOf rdf:resource="http://example.org/chi2025#Study"/>
        <rdfs:comment xml:lang="en">A study in which people interact with a system, prototype, or concept, and their behaviors or experiences are observed or measured.</rdfs:comment>
    </owl:Class>
    


    <!-- http://example.org/chi2025#WizardOfOzStudy -->

    <owl:Class rdf:about="http://example.org/chi2025#WizardOfOzStudy">
        <rdfs:subClassOf rdf:resource="http://example.org/chi2025#Study"/>
        <rdfs:comment xml:lang="en">A study in which a human secretly performs functions of a system component, allowing evaluation of interactions before full automation.</rdfs:comment>
    </owl:Class>
    


    <!-- http://purl.org/ontology/bibo/Article -->

    <owl:Class rdf:about="http://purl.org/ontology/bibo/Article">
        <rdfs:comment xml:lang="en">A bibliographic article, such as a scholarly publication, reused here as the superclass of CHI papers.</rdfs:comment>
    </owl:Class>
    


    <!-- http://schema.org/Organization -->

    <owl:Class rdf:about="http://schema.org/Organization">
        <rdfs:comment xml:lang="en">An organization as defined in schema.org, representing institutions or groups such as companies or universities.</rdfs:comment>
    </owl:Class>
    


    <!-- http://www.w3.org/2004/02/skos/core#Concept -->

    <owl:Class rdf:about="http://www.w3.org/2004/02/skos/core#Concept">
        <rdfs:comment xml:lang="en">A SKOS concept used to represent ideas or topics within a concept scheme.</rdfs:comment>
    </owl:Class>
    


    <!-- http://www.w3.org/2006/vcard/ns#Address -->

    <owl:Class rdf:about="http://www.w3.org/2006/vcard/ns#Address">
        <rdfs:subClassOf>
            <owl:Restriction>
                <owl:onProperty rdf:resource="http://www.w3.org/2006/vcard/ns#country-name"/>
                <owl:someValuesFrom rdf:resource="http://www.w3.org/2001/XMLSchema#string"/>
            </owl:Restriction>
        </rdfs:subClassOf>
        <rdfs:label>Postal Address</rdfs:label>
        <rdfs:comment xml:lang="en">A postal address from the vCard ontology, used to locate organizations or other entities.</rdfs:comment>
    </owl:Class>
    


    <!-- http://www.w3.org/ns/org#Organization -->

    <owl:Class rdf:about="http://www.w3.org/ns/org#Organization">
        <rdfs:subClassOf>
            <owl:Restriction>
                <owl:onProperty rdf:resource="http://www.w3.org/2006/vcard/ns#hasAddress"/>
                <owl:someValuesFrom rdf:resource="http://www.w3.org/2006/vcard/ns#Address"/>
            </owl:Restriction>
        </rdfs:subClassOf>
        <rdfs:label>Organization</rdfs:label>
        <rdfs:comment xml:lang="en">An organization from the W3C ORG ontology, representing institutions or groups that can have postal addresses.</rdfs:comment>
    </owl:Class>
    


    <!-- http://xmlns.com/foaf/0.1/Person -->

    <owl:Class rdf:about="http://xmlns.com/foaf/0.1/Person">
        <rdfs:label>Person</rdfs:label>
        <rdfs:comment xml:lang="en">A person as defined in FOAF, used here to represent authors and other individuals in CHI studies.</rdfs:comment>
    </owl:Class>
    


    <!-- urn:absolute:dev.nemo.inf.ufes.br/hcion/HCIO.owl#Hardware_Equipment -->

    <owl:Class rdf:about="urn:absolute:dev.nemo.inf.ufes.br/hcion/HCIO.owl#Hardware_Equipment">
        <rdfs:comment xml:lang="en">A class from HCIO representing hardware equipment that may be involved in human-computer interaction.</rdfs:comment>
    </owl:Class>
    


    <!-- urn:absolute:dev.nemo.inf.ufes.br/hcion/HCIO.owl#Input_Equipment -->

    <owl:Class rdf:about="urn:absolute:dev.nemo.inf.ufes.br/hcion/HCIO.owl#Input_Equipment">
        <rdfs:comment xml:lang="en">A class from HCIO representing equipment used for user input in interactive computer systems.</rdfs:comment>
    </owl:Class>
    


    <!-- urn:absolute:dev.nemo.inf.ufes.br/hcion/HCIO.owl#Interactive_Computer_System -->

    <owl:Class rdf:about="urn:absolute:dev.nemo.inf.ufes.br/hcion/HCIO.owl#Interactive_Computer_System">
        <rdfs:comment xml:lang="en">A class from HCIO representing an interactive computer system that supports communication with users.</rdfs:comment>
    </owl:Class>
    


    <!-- urn:absolute:dev.nemo.inf.ufes.br/hcion/HCIO.owl#Output_Equipment -->

    <owl:Class rdf:about="urn:absolute:dev.nemo.inf.ufes.br/hcion/HCIO.owl#Output_Equipment">
        <rdfs:comment xml:lang="en">A class from HCIO representing equipment used to present output from an interactive system to users.</rdfs:comment>
    </owl:Class>
    


    <!-- urn:absolute:dev.nemo.inf.ufes.br/hcion/HCIO.owl#User_Goal -->

    <owl:Class rdf:about="urn:absolute:dev.nemo.inf.ufes.br/hcion/HCIO.owl#User_Goal">
        <rdfs:comment xml:lang="en">A class from HCIO representing goals that users aim to achieve through interaction with systems.</rdfs:comment>
    </owl:Class>
    


    <!-- urn:absolute:dev.nemo.inf.ufes.br/hcion/HCIO.owl#User_Intention -->

    <owl:Class rdf:about="urn:absolute:dev.nemo.inf.ufes.br/hcion/HCIO.owl#User_Intention">
        <rdfs:comment xml:lang="en">A class from HCIO representing users&apos; intentions when engaging in human-computer interaction.</rdfs:comment>
    </owl:Class>
    


    <!-- urn:absolute:dev.nemo.inf.ufes.br/hcion/HCIO.owl#User_Interface -->

    <owl:Class rdf:about="urn:absolute:dev.nemo.inf.ufes.br/hcion/HCIO.owl#User_Interface">
        <rdfs:comment xml:lang="en">A class from HCIO representing user interfaces through which people interact with interactive computer systems.</rdfs:comment>
    </owl:Class>
    


    <!-- urn:absolute:dev.nemo.inf.ufes.br/hcion/HCIO.owl#User_Participation -->

    <owl:Class rdf:about="urn:absolute:dev.nemo.inf.ufes.br/hcion/HCIO.owl#User_Participation">
        <rdfs:comment xml:lang="en">A class from HCIO representing the participation of users in interaction or study contexts.</rdfs:comment>
    </owl:Class>
    


    <!-- 
    ///////////////////////////////////////////////////////////////////////////////////////
    //
    // General axioms
    //
    ///////////////////////////////////////////////////////////////////////////////////////
     -->

    <rdf:Description>
        <rdf:type rdf:resource="http://www.w3.org/2002/07/owl#AllDisjointClasses"/>
        <owl:members rdf:parseType="Collection">
            <rdf:Description rdf:about="http://example.org/chi2025#Affiliation"/>
            <rdf:Description rdf:about="http://example.org/chi2025#Author"/>
            <rdf:Description rdf:about="http://example.org/chi2025#DeviceArtifact"/>
            <rdf:Description rdf:about="http://example.org/chi2025#GoalSpecification"/>
            <rdf:Description rdf:about="http://example.org/chi2025#Instrument"/>
            <rdf:Description rdf:about="http://example.org/chi2025#IntentionSpecification"/>
            <rdf:Description rdf:about="http://example.org/chi2025#Measure"/>
            <rdf:Description rdf:about="http://example.org/chi2025#Paper"/>
            <rdf:Description rdf:about="http://example.org/chi2025#ParticipationPattern"/>
            <rdf:Description rdf:about="http://example.org/chi2025#Result"/>
            <rdf:Description rdf:about="http://example.org/chi2025#Session"/>
            <rdf:Description rdf:about="http://example.org/chi2025#Study"/>
            <rdf:Description rdf:about="http://example.org/chi2025#TopicConcept"/>
            <rdf:Description rdf:about="http://example.org/chi2025#Track"/>
        </owl:members>
    </rdf:Description>
</rdf:RDF>



<!-- Generated by the OWL API (version 4.5.29.2024-05-13T12:11:03Z) https://github.com/owlcs/owlapi -->
